test/c/c2rust/test.c
@@ -1,31 +1,17 @@
 #include <stdio.h>
 #include <stdlib.h>
-// void foo(int* abcd) {
-//   int* a = abcd + 0;
-//   int* b = abcd + 8;
-//   int* c = abcd + 16;
-//   int* d = abcd + 24;
-//   b[1] = 42;
-//   abcd[10] = 100;
-//   d[3] = 44;
-// }
+void foo(int* abcd) {
+  int* a = abcd + 0;
+  int* b = abcd + 8;
+  int* c = abcd + 16;
+  int* d = abcd + 24;
+  b[1] = 42;
+  abcd[10] = 100;
+  d[3] = 44;
+}
 int main() {
-  // int abcd[32];
-  // abcd[0] = 1;
-  // abcd[1+2] = 2;
-  // int n = 3;
-  // abcd[n] = 3;
-  // abcd[n+4] = 4;
-  // abcd[1+2+3] = 100;
-  // int* a = abcd + 0;
-  // int* b = abcd + 8;
-  // // foo(abcd);
-  // int* c = abcd + 16;
-  // int* d = abcd + 24;
-  // b[1] = 42;
-  // c[2+n] = 43;
-  // abcd[10] = 100;
-  // d[3] = 44;
+  int abcd[32];
+  foo(abcd);
   int *a = NULL;
   int c=1;
   scanf("%d", &c);
@@ -41,7 +27,6 @@ int main() {
     a[1] = 20;
     free(a);
   }
-  // int *p = rk + 2;
-  // p[1] = 15;
   return 0;
 } 
+
